math start

\(\left(\varepsilon_{1}, \varepsilon_{2}\right) \in \mathbb{R}_{+}^{2}\)

math start

\(\mathbf{E}(\mathbf{r})=\mathbf{E}_{0} e^{i \mathbf{k} \cdot \mathbf{r}}\)

math start

\[\mathbf{k}_{i}=\left(\begin{array}{l}
k_{i x} \\
k_{i y} \\
k_{i z}
\end{array}\right) \quad \mathbf{k}_{r}=\left(\begin{array}{l}
k_{r x} \\
k_{r y} \\
k_{r z}
\end{array}\right) \quad \mathbf{k}_{t}=\left(\begin{array}{l}
k_{t x} \\
k_{t y} \\
k_{t z}
\end{array}\right)\]

math start

\[\mathbf{E}_i(\mathbf{r})=\mathbf{E}_{0} e^{i \mathbf{k_i} \cdot \mathbf{r}},\mathbf{E}_r(\mathbf{r})=r\mathbf{E}_{0} e^{i \mathbf{k_r} \cdot \mathbf{r}},\mathbf{E}_t(\mathbf{r})=t\mathbf{E}_{0} e^{i \mathbf{k_t} \cdot \mathbf{r}}\]

math start

\(\mathbf{E}^\parallel\)

math start

\(z=0\)

math start

\(\mathbf{k}_i,\mathbf{k}_t,\mathbf{k}_r\)

math start

\(\mathbf{k}_\parallel\)

math start

\[\left.e^{i \mathbf{k_i} \cdot \mathbf{r}} + r e^{i \mathbf{k_r} \cdot \mathbf{r}}=t e^{i \mathbf{k_t} \cdot \mathbf{r}}\right|_{z=0}\]

math start

\(k_y=0\)

math start

\[e^{i {k_{ix}x}} + r e^{i{k_{rx}x+k_{ry}y}} = t e^{i{k_{tx}x+k_{ty}y}}, \forall (x,y)\]

math start

\(x=0\)

math start

\[1 + r e^{i{k_{ry}y}} = t e^{i{k_{ty}y}}, \forall y\]

math start

\(r,t\)

math start

\((x,y)\)

math start

\[1 + r \cos(k_{ry}y) = t \cos({k_{ty}y})\]

math start

\(k_{ry}=k_{ty}=0\)

math start

\(k_y=0\)

math start

\[e^{i {k_{ix}x}} + r e^{i{k_{rx}x}} = t e^{i{k_{tx}x}}, \forall x\]

math start

\(e^{-i {k_{ix}x}}\)

math start

\[1 + r e^{i{(k_{rx}-k_{ix})x}} = t e^{i{(k_{tx}-k_{ix})x}}, \forall x\]

math start

\(k_{rx}=k_{tx}=k_{ix}\)

math start

\[\theta_i = \theta_r,\quad n_1\sin \theta_i=n_2\sin \theta_t\]

math start

\(k_{x}, k_{y}\)

math start

\[\mathbf{k}_{i} \cdot \mathbf{k}_{i}=k_{0}^{2} \varepsilon_{i} \quad \Rightarrow k_{i}=k_{0} \sqrt{\varepsilon_{i}}=k_{0} n_{i}\]

math start

\[\left\{\begin{array}{l}k_{i x}=n_{1} k_{0} \sin \theta_{i} \\ k_{r x}=n_{1} k_{0} \sin \theta_{r} \\ k_{t x}=n_{2} k_{0} \sin \theta_{t}\end{array}\right.\]

math start

\[\left\{\begin{array}{c}\theta_{i}=\theta_{r} \\ n_{1} \sin \theta_{i}=n_{2} \sin \theta_{t}\end{array}\right.\]

math start

\((x 0 z) \Rightarrow \mathbf{k}_{1}=k_{1 x} \mathbf{e}_{x}+k_{1 z} \mathbf{e}_{z}\)

math start

\(z=0\)

math start

\(k_{i x}=k_{r x}=k_{t x} \equiv k_{x}\)

math start

\(\mathbf{k} \cdot \mathbf{k}=\varepsilon k_{0}^{2}\)

math start

\[\Rightarrow \left\{\begin{array}{l}
k_{x}^{2}+k_{i z}^{2}=\varepsilon_{1} k_{0}^{2} \quad \Rightarrow k_{i z}=\pm \sqrt{\varepsilon_{1} k_{0}^{2}-k_{x}^{2}}=-k_{r z} \\
k_{x}^{2}+k_{r z}^{2}=\varepsilon_{1} k_{0}^{2} \\
k_{x}^{2}+k_{t z}^{2}=\varepsilon_{2} k_{0}^{2}
\end{array}\right.\]

math start

\(E^y\)

math start

\[1+r =t.\]

math start

\(H^x\)

math start

\(H^x\)

math start

\(\mathbf{k}\times\mathbf{E}= \omega\mathbf{B}= \omega\mu\mathbf{H}\)

math start

\[\omega\mu H_x = k_z E_y\]

math start

\[\frac{k_{iz}}{\mu_1}E_{iy} + \frac{k_{rz}}{\mu_1}E_{ry} = \frac{k_{tz}}{\mu_2}E_{ty}\]

math start

\(k_{rz} = -k_{iz}\)

math start

\[\frac{k_{iz}}{\mu_1} - \frac{k_{iz}}{\mu_1}r = \frac{k_{tz}}{\mu_2}t,\]

math start

\[1 - r = \frac{\mu_1}{\mu_2}\frac{k_{tz}}{k_{iz}}t\]

math start

\[\left\{
\begin{aligned}
1 + r &= t\\
1 - r &= \frac{\mu_1}{\mu_2}\frac{k_{tz}}{k_{iz}}t
\end{aligned}\right.\]

math start

\(r\)

math start

\(t\)

math start

\[t_{12}^s=\frac{2\mu_2 k_{z1}}{\mu_2 k_{z1}+\mu_1k_{z2}},\qquad r_{12}^s=\frac{\mu_2 k_{z1}-\mu_1k_{z2}}{\mu_2 k_{z1}+\mu_1k_{z2}}.\]

math start

\[t_{12}^s=\frac{2}{1+K_s},\qquad r_{12}^s=\frac{1 - K_s}{1 + K_s},\qquad K_s:=\frac{\mu_1}{\mu_2}\frac{k_{z2}}{k_{z1}}\]

math start

\(z\)

math start

\[\begin{aligned}
    \rho_{12}^p & =\frac{\varepsilon_2 k_{z1}-\varepsilon_1k_{z2}}{\varepsilon_2 k_{z1}+\varepsilon_1k_{z2}} = \frac{1-K^p}{1+K^p},%
    & {}& r_{12}^s=\frac{\mu_2 k_{z1}-\mu_1k_{z2}}{\mu_2 k_{z1}+\mu_1k_{z2}} = \frac{1-K^s}{1+K^s}\\
    \tau_{12}^p &=\frac{2\varepsilon_2 k_{z1}}{\varepsilon_2 k_{z1}+\varepsilon_1k_{z2}} = \frac{2}{1+K^p},%
    &{}& t_{12}^s=\frac{2\mu_2 k_{z1}}{\mu_2 k_{z1}+\mu_1k_{z2}} = \frac{2}{1+K^s}
    \end{aligned}\]

math start

\(K^p:= \frac{\varepsilon_1 k_{z2}}{\varepsilon_2 k_{z1}}\)

math start

\(K^s:= \frac{ k_{z2}}{ k_{z1}}\)

math start

\(\mu=1\)

math start

\[r_{ij}=-r_{ji}.\]

math start

\(\theta\)

math start

\[r^{p}=\frac{n_{2} \cos \theta-n_{1} \sqrt{1-\frac{n_{1}^{2}}{n_{2}^{2}} \sin ^{2} \theta}}{n_{2} \cos \theta+n_{1} \sqrt{1-\frac{n_{1}^{2}}{n_{2}^{2}} \sin ^{2} \theta}}\]
